Finish fbs full congruence

src/Core_Erlang_Full_Equivalence.v
@@ -136,6 +136,38 @@ Proof.
   * apply H0 in H1. apply H in H1. auto.
 Qed.
 
+Definition fully_equivalent_case l1 l2 :=
+forall env eff res eff' id1 id2 vals,
+  (exists clock, fbs_case l1 env id1 eff vals (fbs_expr clock) = Result id2 res eff')
+<->
+  (exists clock, fbs_case l2 env id1 eff vals (fbs_expr clock) = Result id2 res eff').
+
+Theorem fully_equivalent_case_refl {l} :
+  fully_equivalent_case l l.
+Proof.
+  intros. unfold fully_equivalent_case. split; intros.
+  * auto.
+  * auto.
+Qed.
+
+Theorem fully_equivalent_case_sym {l1 l2} :
+  fully_equivalent_case l1 l2 -> fully_equivalent_case l2 l1.
+Proof.
+  unfold fully_equivalent_case; intros.
+  split; apply H.
+Qed.
+
+Theorem fully_equivalent_case_trans {l1 l2 l3} :
+  fully_equivalent_case l1 l2 -> fully_equivalent_case l2 l3
+->
+  fully_equivalent_case l1 l3.
+Proof.
+  unfold fully_equivalent_case; intros.
+  split; intros.
+  * apply H in H1. apply H0 in H1. auto.
+  * apply H0 in H1. apply H in H1. auto.
+Qed.
+
 (** If all elements are equivalent in a list, then the lists are equivalent too
   * ATTENTION: does not work in the opposite direction 
   * *)
@@ -235,11 +267,86 @@ all: try lia.
 intros. apply (H0 (S i)). simpl. lia.
 Qed.
 
+Theorem fully_equivalent_elements_case (l l' : list (list Pattern * Expression * Expression )) :
+  length l = length l' ->
+  ((forall i, i < length l -> fully_equivalent_expr (nth i (map snd l) ErrorExp)
+                                                   (nth i (map snd l') ErrorExp) /\
+                             fully_equivalent_expr (nth i (map snd (map fst l)) ErrorExp)
+                                                   (nth i (map snd (map fst l')) ErrorExp)
+                   /\ nth i (map fst (map fst l)) [] = nth i (map fst (map fst l')) []))
+->
+  fully_equivalent_case l l'
+.
+Proof.
+  generalize dependent l'. induction l; intros.
+  * apply eq_sym, length_zero_iff_nil in H. subst. split; intros; assumption.
+  * pose (EE := element_exist _ _ H). destruct EE, H1. subst. inversion H.
+    pose (F := H0 0 (Nat.lt_0_succ _)). simpl in F.
+    epose (IH := IHl _ H2 _). Unshelve. 2: { intros. apply (H0 (S i)). simpl. lia. }
+    split; intros; destruct H1; simpl in H1.
+    - destruct a, p. destruct (match_valuelist_to_patternlist vals l0) eqn:D1.
+      + destruct (fbs_expr x1 (add_bindings (match_valuelist_bind_patternlist vals l0) env) id1 e0
+         eff) eqn:D2.
+         destruct res0. destruct v. congruence. destruct v0. 2: congruence. 3-4: congruence.
+         ** destruct (((id =? id1) && list_eqb effect_eqb eff eff0)%bool) eqn:D3. 2: congruence.
+            apply andb_prop in D3. destruct D3. apply Nat.eqb_eq in H3.
+            apply effect_list_eqb_eq in H4. subst.
+            destruct v; try congruence. destruct l1; try congruence.
+            destruct (s =? "true")%string eqn:D4.
+            -- apply eqb_eq in D4. subst.
+               destruct F, H4. destruct x, p. simpl in H3, H4, H5.
+               epose (P := H4 _ _ _ _ _ _). destruct P. pose (P1 := H6 (ex_intro _ _ D2)).
+               epose (P := H3 _ _ _ _ _ _). destruct P. pose (P2 := H8 (ex_intro _ _ H1)).
+               destruct P1, P2. exists (x + x2). simpl. subst. rewrite D1.
+               erewrite (bigger_clock_expr _ _ H10). rewrite Nat.eqb_refl, effect_list_eqb_refl.
+               simpl. eapply (bigger_clock_expr _ _ H11). Unshelve. all: lia.
+            -- destruct (s =? "false")%string eqn:D5. 2: congruence.
+               apply eqb_eq in D5. subst.
+               destruct F, H4. destruct x, p. simpl in H3, H4, H5.
+               epose (P := H4 _ _ _ _ _ _). destruct P. pose (P1 := H6 (ex_intro _ _ D2)).
+               epose (P := IH _ _ _ _ _ _ _). destruct P. pose (P2 := H8 (ex_intro _ _ H1)).
+               clear IH. destruct P1, P2. exists (x + x2). simpl. subst. rewrite D1.
+               erewrite (bigger_clock_expr _ _ H10). rewrite Nat.eqb_refl, effect_list_eqb_refl.
+               simpl. eapply (bigger_clock_case _ H11 _). Unshelve. all: lia.
+         ** congruence.
+       + epose (P := IH _ _ _ _ _ _ _). destruct P. pose (P2 := H3 (ex_intro _ _ H1)).
+         clear IH. destruct P2. exists x2. simpl. destruct F, H7. destruct x, p.
+         simpl in H6, H7, H8. subst. rewrite D1. assumption.
+    - destruct x, p. destruct (match_valuelist_to_patternlist vals l0) eqn:D1.
+      + destruct (fbs_expr x1 (add_bindings (match_valuelist_bind_patternlist vals l0) env) id1 e0
+         eff) eqn:D2.
+         destruct res0. destruct v. congruence. destruct v0. 2: congruence. 3-4: congruence.
+         ** destruct (((id =? id1) && list_eqb effect_eqb eff eff0)%bool) eqn:D3. 2: congruence.
+            apply andb_prop in D3. destruct D3. apply Nat.eqb_eq in H3.
+            apply effect_list_eqb_eq in H4. subst.
+            destruct v; try congruence. destruct l1; try congruence.
+            destruct (s =? "true")%string eqn:D4.
+            -- apply eqb_eq in D4. subst.
+               destruct F, H4. destruct a, p. simpl in H3, H4, H5.
+               epose (P := H4 _ _ _ _ _ _). destruct P. pose (P1 := H7 (ex_intro _ _ D2)).
+               epose (P := H3 _ _ _ _ _ _). destruct P. pose (P2 := H9 (ex_intro _ _ H1)).
+               destruct P1, P2. exists (x + x2). simpl. subst. rewrite D1.
+               erewrite (bigger_clock_expr _ _ H10). rewrite Nat.eqb_refl, effect_list_eqb_refl.
+               simpl. eapply (bigger_clock_expr _ _ H11). Unshelve. all: lia.
+            -- destruct (s =? "false")%string eqn:D5. 2: congruence.
+               apply eqb_eq in D5. subst.
+               destruct F, H4. destruct a, p. simpl in H3, H4, H5.
+               epose (P := H4 _ _ _ _ _ _). destruct P. pose (P1 := H7 (ex_intro _ _ D2)).
+               epose (P := IH _ _ _ _ _ _ _). destruct P. pose (P2 := H9 (ex_intro _ _ H1)).
+               clear IH. destruct P1, P2. exists (x + x2). simpl. subst. rewrite D1.
+               erewrite (bigger_clock_expr _ _ H10). rewrite Nat.eqb_refl, effect_list_eqb_refl.
+               simpl. eapply (bigger_clock_case _ H11 _). Unshelve. all: lia.
+         ** congruence.
+       + epose (P := IH _ _ _ _ _ _ _). destruct P. pose (P2 := H4 (ex_intro _ _ H1)).
+         clear IH. destruct P2. exists x. simpl. destruct F, H7. destruct a, p.
+         simpl in H6, H7, H8. subst. rewrite D1. assumption.
+Qed.
+
 End equivalence_relation.
 
 Section congruence.
 
-Theorem ECons_congr hd tl : forall hd' tl',
+Theorem ECons_full_cong hd tl : forall hd' tl',
   fully_equivalent_expr hd hd' -> fully_equivalent_expr tl tl'
 ->
   fully_equivalent_single (ECons hd tl) (ECons hd' tl').
@@ -258,13 +365,13 @@ Proof.
     destruct res0. destruct v. congruence. destruct v0. 2: congruence. 3-4: congruence.
     - destruct (fbs_expr x env id0 hd0 eff0) eqn:D2.
       destruct res0. destruct v0. congruence. destruct v1. 2: congruence. 3-4: congruence.
-      + inversion H1. subst. epose (D1' := H0 _ _ _ _ _ _). destruct D1'. epose (H2 (ex_intro (fun x => fbs_expr x env id tl0 eff = Result id0 (inl [v]) eff0) x D1)).
-        epose (D2' := H _ _ _ _ _ _). destruct D2'. epose (H4 (ex_intro (fun x => fbs_expr x env id0 hd0 eff0 = Result id' (inl [v0]) eff') x D2)). destruct e, e0.
+      + inversion H1. subst. epose (D1' := H0 _ _ _ _ _ _). destruct D1'. epose (H2 (ex_intro _ x D1)).
+        epose (D2' := H _ _ _ _ _ _). destruct D2'. epose (H4 (ex_intro _ x D2)). destruct e, e0.
         exists (S (x0 + x1)). simpl. erewrite (bigger_clock_expr _ _ H6), (bigger_clock_expr _ _ H7). reflexivity.
-      + inversion H1. subst. epose (D1' := H0 _ _ _ _ _ _). destruct D1'. epose (H2 (ex_intro (fun x => fbs_expr x env id tl0 eff = Result id0 (inl [v]) eff0) x D1)).
-        epose (D2' := H _ _ _ _ _ _). destruct D2'. epose (H4 (ex_intro (fun x => fbs_expr x env id0 hd0 eff0 = Result id' (inr e) eff') x D2)). destruct e0, e1.
+      + inversion H1. subst. epose (D1' := H0 _ _ _ _ _ _). destruct D1'. epose (H2 (ex_intro _ x D1)).
+        epose (D2' := H _ _ _ _ _ _). destruct D2'. epose (H4 (ex_intro _ x D2)). destruct e0, e1.
         exists (S (x0 + x1)). simpl. erewrite (bigger_clock_expr _ _ H6), (bigger_clock_expr _ _ H7). reflexivity.
-    - inversion H1. subst. epose (D1' := H0 _ _ _ _ _ _). destruct D1'. epose (H2 (ex_intro (fun x => fbs_expr x env id tl0 eff = Result id' (inr e) eff') x D1)).
+    - inversion H1. subst. epose (D1' := H0 _ _ _ _ _ _). destruct D1'. epose (H2 (ex_intro _ x D1)).
       destruct e0. exists (S x0). simpl. rewrite H4. auto.
   }
   split; intros.
@@ -275,7 +382,7 @@ Unshelve.
 all: lia.
 Qed.
 
-Theorem ETuple_congr (l : list Expression) : forall (l' : list Expression),
+Theorem ETuple_full_cong (l : list Expression) : forall (l' : list Expression),
   fully_equivalent_exprlist l l'
 ->
   fully_equivalent_single (ETuple l) (ETuple l').
@@ -292,469 +399,340 @@ Proof.
     destruct (fbs_values (fbs_expr x) env id l0 eff) eqn:D.
     destruct res0. 3-4: congruence.
     * inversion H0. subst. epose (E := H _ _ _ _ _ _). destruct E.
-      pose (E := H1 (ex_intro (fun x => fbs_values (fbs_expr x) env id l0 eff = Result id' (inl v) eff') x D)). destruct E. exists (S x0). simpl. rewrite H3. auto.
+      pose (E := H1 (ex_intro _ x D)). destruct E. exists (S x0). simpl. rewrite H3. auto.
     * inversion H0. subst. epose (E := H _ _ _ _ _ _). destruct E.
-      pose (E := H1 (ex_intro (fun x => fbs_values (fbs_expr x) env id l0 eff = Result id' (inr e) eff') x D)). destruct E. exists (S x0). simpl. rewrite H3. auto.
+      pose (E := H1 (ex_intro _ x D)). destruct E. exists (S x0). simpl. rewrite H3. auto.
   }
   split; intros.
   * eapply A. exact H. auto.
   * eapply A. exact (fully_equivalent_exprlist_sym H). exact H0.
 Qed.
 
-Theorem ECall_congr (f : string) (l : list Expression) : forall (l' : list Expression),
-  length l = length l' ->
-  (forall i, i < length l -> fully_equivalent (nth i l ErrorExp) (nth i l' ErrorExp))
+Theorem ECall_full_cong (f : string) (l : list Expression) : forall (l' : list Expression),
+  fully_equivalent_exprlist l l'
 ->
   fully_equivalent_single (ECall f l) (ECall f l').
 Proof.
   assert (A : forall f (l l' : list Expression) env id eff id' res eff',
-  length l = length l' ->
-  (forall i, i < length l -> fully_equivalent (nth i l ErrorExp) (nth i l' ErrorExp))
+  fully_equivalent_exprlist l l'
   ->
-  |env, id, ECall f l, eff| -s> |id', res, eff'|
+  (exists clock, fbs_single clock env id (ECall f l) eff = Result id' res eff')
   ->
-  |env, id, ECall f l', eff| -s> |id', res, eff'|). {
-  intros. unfold fully_equivalent, fully_equivalent_single in *.
-  * inversion H1; subst; rewrite H in *.
-    - eapply eval_call.
-      + exact H4.
-      + exact H5.
-      + exact H6.
-      + intros. pose (H7 i H2). apply H0 in e. 2: auto. auto.
-      + auto.
-      + auto.
-    - eapply eval_call_ex.
-      + exact H4.
-      + reflexivity.
-      + exact H6.
-      + exact H7.
-      + intros. pose (H10 j H2). apply H0 in e. 2: lia. auto.
-      + apply H0 in H15. auto. lia.
+  (exists clock, fbs_single clock env id (ECall f l') eff = Result id' res eff')). 
+  {
+    intros. destruct H0, x. inversion H0. simpl in H0.
+    destruct (fbs_values (fbs_expr x) env id l0 eff) eqn:D.
+    destruct res0. 3-4: congruence.
+    all: epose (P := H _ _ _ _ _ _); destruct P; pose (P := H1 (ex_intro _ x D));
+      destruct P; exists (S x0); simpl; rewrite H3; assumption.
   }
   split; intros.
-  * eapply A. exact H. auto. auto.
-  * eapply A. symmetry. exact H. intros. rewrite <- H in *.
-    apply fully_equivalent_sym. auto. auto.
+  * eapply A. exact H. auto.
+  * eapply A. exact (fully_equivalent_exprlist_sym H). exact H0.
 Qed.
 
-Theorem EPrimOp_congr (f : string) (l : list Expression) : forall (l' : list Expression),
-  length l = length l' ->
-  (forall i, i < length l -> fully_equivalent (nth i l ErrorExp) (nth i l' ErrorExp))
+Theorem EPrimOp_full_cong (f : string) (l : list Expression) : forall (l' : list Expression),
+  fully_equivalent_exprlist l l'
 ->
   fully_equivalent_single (EPrimOp f l) (EPrimOp f l').
 Proof.
   assert (A : forall f (l l' : list Expression) env id eff id' res eff',
-  length l = length l' ->
-  (forall i, i < length l -> fully_equivalent (nth i l ErrorExp) (nth i l' ErrorExp))
+  fully_equivalent_exprlist l l'
   ->
-  |env, id, EPrimOp f l, eff| -s> |id', res, eff'|
+  (exists clock, fbs_single clock env id (EPrimOp f l) eff = Result id' res eff')
   ->
-  |env, id, EPrimOp f l', eff| -s> |id', res, eff'|). {
-  intros. unfold fully_equivalent, fully_equivalent_single in *.
-  * inversion H1; subst; rewrite H in *.
-    - eapply eval_primop.
-      + exact H4.
-      + exact H5.
-      + exact H6.
-      + intros. pose (H7 i H2). apply H0 in e. 2: auto. auto.
-      + auto.
-      + auto.
-    - eapply eval_primop_ex.
-      + exact H4.
-      + reflexivity.
-      + exact H6.
-      + exact H7.
-      + intros. pose (H10 j H2). apply H0 in e. 2: lia. auto.
-      + apply H0 in H15. auto. lia.
+  (exists clock, fbs_single clock env id (EPrimOp f l') eff = Result id' res eff')). 
+  {
+    intros. destruct H0, x. inversion H0. simpl in H0.
+    destruct (fbs_values (fbs_expr x) env id l0 eff) eqn:D.
+    destruct res0. 3-4: congruence.
+    all: epose (P := H _ _ _ _ _ _); destruct P; pose (P := H1 (ex_intro _ x D));
+      destruct P; exists (S x0); simpl; rewrite H3; assumption.
   }
   split; intros.
-  * eapply A. exact H. auto. auto.
-  * eapply A. symmetry. exact H. intros. rewrite <- H in *.
-    apply fully_equivalent_sym. auto. auto.
+  * eapply A. exact H. auto.
+  * eapply A. exact (fully_equivalent_exprlist_sym H). exact H0.
 Qed.
 
-Theorem EApp_congr (exp : Expression) (l : list Expression) : forall (exp' : Expression) (l' : list Expression),
-  length l = length l' ->
-  fully_equivalent exp exp' ->
-  (forall i, i < length l -> fully_equivalent (nth i l ErrorExp) (nth i l' ErrorExp))
+Theorem EApp_full_cong (exp : Expression) (l : list Expression) : forall (exp' : Expression) (l' : list Expression),
+  fully_equivalent_expr exp exp' ->
+  fully_equivalent_exprlist l l'
 ->
   fully_equivalent_single (EApp exp l) (EApp exp' l').
 Proof.
   assert (A : forall exp exp' (l l' : list Expression) env id eff id' res eff',
-    length l = length l' ->
-    fully_equivalent exp exp' ->
-    (forall i, i < length l -> fully_equivalent (nth i l ErrorExp) (nth i l' ErrorExp))
+    fully_equivalent_expr exp exp' ->
+    fully_equivalent_exprlist l l'
     ->
-    |env, id, EApp exp l, eff| -s> |id', res, eff'|
+    (exists clock, fbs_single clock env id (EApp exp l) eff = Result id' res eff')
     ->
-    |env, id, EApp exp' l', eff| -s> |id', res, eff'|).
+    (exists clock, fbs_single clock env id (EApp exp' l') eff = Result id' res eff')).
   {
-    unfold fully_equivalent.
-    intros. remember (EApp exp0 l0) as appl.
-    induction H2; inversion Heqappl; subst.
-    * eapply eval_app; rewrite H in *.
-      - exact H2.
-      - apply H0. exact H3.
-      - auto.
-      - exact H5.
-      - exact H6.
-      - intros. pose (H7 i H9). apply H1. auto. auto.
-      - auto.
-    * eapply eval_app_closure_ex. apply H0. exact H2.
-    * eapply eval_app_param_ex; rewrite H in *.
-      - exact H2.
-      - reflexivity.
-      - exact H4.
-      - exact H5.
-      - apply H0. auto. exact H6.
-      - intros. pose (H7 j H3). apply H1. lia. auto.
-      - apply H1. lia. auto.
-    * eapply eval_app_badfun_ex; rewrite H in *.
-      - exact H2.
-      - exact H3.
-      - exact H4.
-      - apply H0. auto. exact H5.
-      - intros. pose (H6 j H8). apply H1. lia. auto.
-      - congruence.
-      - auto.
-      - auto.
-    * eapply eval_app_badarity_ex; rewrite H in *.
-      - exact H2.
-      - exact H3.
-      - exact H4.
-      - apply H0. auto. exact H5.
-      - intros. pose (H6 j H8). apply H1. lia. auto.
-      - congruence.
-      - auto.
-      - auto.
+    intros. destruct H1, x. inversion H1. simpl in H1.
+    destruct (fbs_expr x env id exp0 eff) eqn:D1.
+    destruct res0. destruct v. congruence. destruct v0. 2: congruence. 3-4: congruence.
+    * destruct (fbs_values (fbs_expr x) env id0 l0 eff0) eqn:D2.
+      destruct res0. 3-4: congruence.
+      - epose (P := H _ _ _ _ _ _); destruct P; pose (P := H2 (ex_intro _ x D1)); destruct P;
+        epose (P := H0 _ _ _ _ _ _); destruct P; pose (P := H5 (ex_intro _ x D2)); destruct P.
+        destruct v.
+        + exists (S (x0 + x1)); simpl; eapply bigger_clock_list in H7;
+          try (erewrite (bigger_clock_expr _ _ H4), H7; assumption).
+          lia.
+          intros; apply clock_increase_expr; auto.
+        + exists (S (x0 + x1)); simpl; eapply bigger_clock_list in H7;
+          try (erewrite (bigger_clock_expr _ _ H4), H7; assumption).
+          lia.
+          intros; apply clock_increase_expr; auto.
+        + destruct (length vl =? length v0) eqn:D3.
+          ** exists (S (x0 + x1 + x)). simpl; eapply bigger_clock_list in H7.
+             erewrite (bigger_clock_expr _ _ H4), H7, D3, (bigger_clock_expr _ _ H1). auto.
+             lia.
+             intros; apply clock_increase_expr; auto.
+          ** exists (S (x0 + x1)); simpl; eapply bigger_clock_list in H7.
+             erewrite (bigger_clock_expr _ _ H4), H7, D3. assumption.
+             lia.
+             intros; apply clock_increase_expr; auto.
+        + exists (S (x0 + x1)); simpl; eapply bigger_clock_list in H7;
+          try (erewrite (bigger_clock_expr _ _ H4), H7; assumption).
+          lia.
+          intros; apply clock_increase_expr; auto.
+        + exists (S (x0 + x1)); simpl; eapply bigger_clock_list in H7;
+          try (erewrite (bigger_clock_expr _ _ H4), H7; assumption).
+          lia.
+          intros; apply clock_increase_expr; auto.
+        + exists (S (x0 + x1)); simpl; eapply bigger_clock_list in H7;
+          try (erewrite (bigger_clock_expr _ _ H4), H7; assumption).
+          lia.
+          intros; apply clock_increase_expr; auto.
+      - epose (P := H _ _ _ _ _ _). destruct P. pose (P := H2 (ex_intro _ x D1)). destruct P.
+        epose (P := H0 _ _ _ _ _ _). destruct P. pose (P := H5 (ex_intro _ x D2)). destruct P.
+        exists (S (x0 + x1)). simpl. eapply bigger_clock_list in H7.
+        erewrite (bigger_clock_expr _ _ H4), H7. assumption.
+        lia. intros. apply clock_increase_expr. auto.
+    * epose (P := H _ _ _ _ _ _). destruct P. pose (P := H2 (ex_intro _ x D1)).
+      destruct P. exists (S x0). simpl. rewrite H4. assumption.
   }
-  intros. split.
-  * apply A; auto.
-  * apply A; try lia.
-    apply fully_equivalent_sym. auto.
-    intros. apply fully_equivalent_sym. apply H1. lia.
+  split; intros.
+  * eapply A. exact H. exact H0. auto.
+  * eapply A. exact (fully_equivalent_expr_sym H). exact (fully_equivalent_exprlist_sym H0). exact H1.
+Unshelve.
+all: lia.
 Qed.
 
-Lemma match_clause_ith l : forall vals i gg ee bb,
-  match_clause vals l i = Some (gg,ee,bb)
-->
-  gg = nth i (map snd (map fst l)) ErrorExp /\
-  ee = nth i (map snd l) ErrorExp /\
-  bb = match_valuelist_bind_patternlist vals (nth i (map fst (map fst l)) []).
-Proof.
-  induction l; intros.
-  * inversion H.
-  * destruct i.
-    - destruct a. destruct p. simpl. simpl in H.
-      destruct (match_valuelist_to_patternlist vals l0); inversion H. auto.
-    - simpl in H. destruct a, p.
-      simpl. pose (IHl _ _ _ _ _ H). exact a.
-Qed.
-
-Theorem case_congr_helper (l l' : list (list Pattern * Expression * Expression)) vals j gg ee bb:
-length l = length l' ->
-((forall i, i < length l -> fully_equivalent (nth i (map snd l) ErrorExp)
-                                                   (nth i (map snd l') ErrorExp) /\
-                             fully_equivalent (nth i (map snd (map fst l)) ErrorExp)
-                                                   (nth i (map snd (map fst l')) ErrorExp)
-                   /\ nth i (map fst (map fst l)) [] = nth i (map fst (map fst l')) [])) ->
- match_clause vals l j = Some (gg, ee, bb)
-->
- match_clause vals l' j = Some (nth j (map snd (map fst l')) ErrorExp, nth j (map snd l') ErrorExp, bb).
-Proof.
-  generalize dependent l'. generalize dependent j.
-  induction l; intros.
-  * inversion H1.
-  * pose (element_exist _ _ H). destruct e. destruct H2. subst.
-    inversion H.
-    destruct j.
-    - simpl. simpl in H1. destruct a, p, x, p.
-      pose (H0 0 (Nat.lt_0_succ _)). destruct a. destruct H4.
-      simpl in H2, H4, H5. subst.
-      destruct (match_valuelist_to_patternlist vals l1).
-      + simpl. inversion H1. auto.
-      + congruence.
-    - simpl. simpl in H1. destruct a, p, x, p.
-      apply IHl. auto.
-      intros. epose (H0 (S i) _). simpl in a. exact a. Unshelve. 2: simpl; lia.
-      auto.
-Qed.
-
-Theorem ECase_congr (exp : Expression) (l : list (list Pattern * Expression * Expression)) : forall (exp' : Expression) (l' : list (list Pattern * Expression * Expression)),
-  length l = length l' ->
-  fully_equivalent exp exp' ->
-  (forall i, i < length l -> fully_equivalent (nth i (map snd l) ErrorExp)
-                                                   (nth i (map snd l') ErrorExp) /\
-                             fully_equivalent (nth i (map snd (map fst l)) ErrorExp)
-                                                   (nth i (map snd (map fst l')) ErrorExp)
-                   /\ nth i (map fst (map fst l)) [] = nth i (map fst (map fst l')) [])
+Theorem ECase_full_cong (exp : Expression) (l : list (list Pattern * Expression * Expression)) : forall (exp' : Expression) (l' : list (list Pattern * Expression * Expression)),
+  fully_equivalent_expr exp exp' ->
+  fully_equivalent_case l l'
 ->
   fully_equivalent_single (ECase exp l) (ECase exp' l').
 Proof.
-  intros. unfold fully_equivalent, fully_equivalent_single in *.
-  split; intros; inversion H2; subst.
-  * eapply eval_case; rewrite H in *.
-    - apply H0. exact H5.
-    - exact H6.
-    - apply case_congr_helper with (l' := l') in H7.
-      3: unfold fully_equivalent; rewrite H; exact H1.
-      exact H7.
-      auto.
-    - intros. assert (match_clause vals l' j = Some (gg, ee, bb)). { auto. }
-      apply match_clause_ith in H9. destruct H9. destruct H10. subst.
-      apply case_congr_helper with (l' := l) in H4. 2: auto.
-      pose (H8 j H3 _ _ _ H4). epose (H1 j _). Unshelve. 3: lia. destruct a.
-      apply H10. exact e.
-      intros. split. 2: split.
-      + apply fully_equivalent_sym. epose (H1 i0 _). Unshelve. 2: lia. destruct a.
-        unfold fully_equivalent.
-        intros. apply H10.
-      + apply fully_equivalent_sym. epose (H1 i0 _). Unshelve. 2: lia. destruct a.
-        unfold fully_equivalent.
-        intros. apply H12.
-      + epose (H1 i0 _). Unshelve. 2: lia. destruct a.
-        destruct H12. auto.
-    - apply match_clause_ith in H7. destruct H7, H4. subst.
-      apply H1. auto. auto.
-    - apply match_clause_ith in H7. destruct H7, H4. subst.
-      apply H1. auto. auto.
-  * eapply eval_case_pat_ex. apply H0. auto.
-  * eapply eval_case_clause_ex.
-    - apply H0. exact H7.
-    - intros. assert (match_clause vals l' j = Some (gg, ee, bb)). { auto. }
-      apply match_clause_ith in H5. destruct H5. destruct H6. subst.
-      apply case_congr_helper with (l' := l) in H4.
-      rewrite H in *. 2: auto.
-      pose (H12 j H3 _ _ _ H4). epose (H1 j _). Unshelve. 3: lia. destruct a.
-      apply H6. exact e.
-      intros. split. 2: split.
-      + apply fully_equivalent_sym. epose (H1 i _). Unshelve. 2: lia. destruct a.
-        unfold fully_equivalent.
-        intros. apply H6.
-      + apply fully_equivalent_sym. epose (H1 i _). Unshelve. 2: lia. destruct a.
-        unfold fully_equivalent.
-        intros. apply H8.
-      + epose (H1 i _). Unshelve. 2: lia. destruct a.
-        destruct H8. auto.
-  * eapply eval_case; rewrite <- H in *.
-    - apply H0. exact H5.
-    - exact H6.
-    - apply case_congr_helper with (l' := l) in H7. 2: lia.
-      exact H7.
-      rewrite <- H. intros.
-      split. 2: split.
-      + apply fully_equivalent_sym. pose (H1 i0 H3). unfold fully_equivalent.
-        apply a.
-      + apply fully_equivalent_sym. pose (H1 i0 H3). unfold fully_equivalent.
-        apply a.
-      + pose (H1 i0 H3). unfold fully_equivalent. destruct a. destruct H9.
-        symmetry. apply H10.
-    - intros. assert (match_clause vals l j = Some (gg, ee, bb)). { auto. }
-      apply match_clause_ith in H9. destruct H9. destruct H10. subst.
-      apply case_congr_helper with (l' := l') in H4. 2: auto.
-      pose (H8 j H3 _ _ _ H4). epose (H1 j _). Unshelve. 3: lia. destruct a.
-      apply H10. exact e.
-      intros. split. 2: split.
-      + apply fully_equivalent_sym. epose (H1 i0 _). Unshelve. 2: lia. destruct a.
-        unfold fully_equivalent. symmetry.
-        intros. apply H10.
-      + apply fully_equivalent_sym. epose (H1 i0 _). Unshelve. 2: lia. destruct a.
-        unfold fully_equivalent.
-        intros. symmetry. apply H12.
-      + epose (H1 i0 _). Unshelve. 2: lia. destruct a.
-        destruct H12. auto.
-    - apply match_clause_ith in H7. destruct H7, H4. subst.
-      apply H1. auto. auto.
-    - apply match_clause_ith in H7. destruct H7, H4. subst.
-      apply H1. auto. auto.
-  * eapply eval_case_pat_ex. apply H0. auto.
-  * eapply eval_case_clause_ex.
-    - apply H0. exact H7.
-    - intros. assert (match_clause vals l j = Some (gg, ee, bb)). { auto. }
-      apply match_clause_ith in H5. destruct H5. destruct H6. subst.
-      apply case_congr_helper with (l' := l') in H4. 2: auto.
-      rewrite H in *.
-      pose (H12 j H3 _ _ _ H4). epose (H1 j _). Unshelve. 3: lia. destruct a.
-      apply H6. exact e.
-      intros. split. 2: split.
-      + apply fully_equivalent_sym. epose (H1 i _). Unshelve. 2: lia. destruct a.
-        unfold fully_equivalent.
-        intros. symmetry. apply H6.
-      + apply fully_equivalent_sym. epose (H1 i _). Unshelve. 2: lia. destruct a.
-        unfold fully_equivalent.
-        intros. symmetry. apply H8.
-      + epose (H1 i _). Unshelve. 2: lia. destruct a.
-        destruct H8. auto.
+  assert (A : forall exp exp' l l' env id eff id' res eff',
+    fully_equivalent_expr exp exp' ->
+    fully_equivalent_case l l' ->
+    (exists clock, fbs_single clock env id (ECase exp l) eff = Result id' res eff')
+   ->
+    (exists clock, fbs_single clock env id (ECase exp' l') eff = Result id' res eff')
+  ).
+  {
+    intros. destruct H1, x. inversion H1. simpl in H1.
+    destruct (fbs_expr x env id exp0 eff) eqn:D.
+    destruct res0. 3-4: congruence.
+    * epose (P := H _ _ _ _ _ _). destruct P. pose (P := H2 (ex_intro _ x D)). destruct P.
+      epose (P := H0 _ _ _ _ _ _ _). destruct P. pose (P := H5 (ex_intro _ x H1)). destruct P.
+      exists (S (x0 + x1)). simpl. eapply bigger_clock_case in H7.
+      erewrite (bigger_clock_expr _ _ H4). exact H7. lia.
+      Unshelve. lia.
+    * epose (P := H _ _ _ _ _ _). destruct P. pose (P := H2 (ex_intro _ x D)). destruct P.
+      exists (S x0). simpl. rewrite H4. auto.
+  }
+  split; intros.
+  * eapply A. exact H. exact H0. auto.
+  * eapply A. exact (fully_equivalent_expr_sym H). exact (fully_equivalent_case_sym H0). auto.
 Qed.
 
-Theorem ELet_congr (e1 e2 : Expression) vl : forall (e1' e2' : Expression),
-  fully_equivalent e1 e1' ->
-  fully_equivalent e2 e2'
+Theorem ELet_full_cong (e1 e2 : Expression) vl : forall (e1' e2' : Expression),
+  fully_equivalent_expr e1 e1' ->
+  fully_equivalent_expr e2 e2'
 ->
   fully_equivalent_single (ELet vl e1 e2) (ELet vl e1' e2').
 Proof.
-  intros. unfold fully_equivalent, fully_equivalent_single in *.
+  assert (A : forall env id id' res eff eff' e1 e1' e2 e2',
+    fully_equivalent_expr e1 e1' ->
+    fully_equivalent_expr e2 e2' ->
+    (exists clock, fbs_single clock env id (ELet vl e1 e2) eff = Result id' res eff')
+   ->
+    (exists clock, fbs_single clock env id (ELet vl e1' e2') eff = Result id' res eff')
+  ).
+  {
+    intros.
+    destruct H1. destruct x. inversion H1. simpl in H1.
+    destruct (fbs_expr x env id e0 eff) eqn:D1.
+    destruct res0.
+    destruct (Datatypes.length v =? Datatypes.length vl) eqn:D2. 2, 4-5: congruence.
+    * epose (P := H _ _ _ _ _ _). destruct P. pose (P1 := H2 (ex_intro _ _ D1)).
+      epose (P := H0 _ _ _ _ _ _). destruct P. pose (P2 := H4 (ex_intro _ _ H1)).
+      destruct P1, P2. exists (S (x0 + x1)). simpl.
+      erewrite (bigger_clock_expr _ _ H6), (bigger_clock_expr _ _ H7), D2. auto.
+      Unshelve. all: lia.
+    * epose (P := H _ _ _ _ _ _). destruct P. pose (P1 := H2 (ex_intro _ _ D1)). destruct P1.
+      exists (S x0). simpl. erewrite (bigger_clock_expr _ _ H4). auto. Unshelve. lia.
+  }
   split; intros.
-  * inversion H1; subst.
-    - eapply eval_let. apply H. exact H7. auto. apply H0. exact H13.
-    - eapply eval_let_ex. apply H. auto.
-  * inversion H1; subst.
-    - eapply eval_let. apply H. exact H7. auto. apply H0. exact H13.
-    - eapply eval_let_ex. apply H. auto.
+  * eapply A. exact H. exact H0. auto.
+  * eapply A. exact (fully_equivalent_expr_sym H). exact (fully_equivalent_expr_sym H0). auto.
 Qed.
 
-Theorem ESeq_congr (e1 e2 : Expression) (l : list Expression) : forall (e1' e2' : Expression),
-  fully_equivalent e1 e1' ->
-  fully_equivalent e2 e2'
+Theorem ESeq_full_cong (e1 e2 : Expression) (l : list Expression) : forall (e1' e2' : Expression),
+  fully_equivalent_expr e1 e1' ->
+  fully_equivalent_expr e2 e2'
 ->
   fully_equivalent_single (ESeq e1 e2) (ESeq e1' e2').
 Proof.
-  intros. unfold fully_equivalent, fully_equivalent_single in *.
+  assert (A : forall env id id' res eff eff' e1 e1' e2 e2',
+    fully_equivalent_expr e1 e1' ->
+    fully_equivalent_expr e2 e2' ->
+    (exists clock, fbs_single clock env id (ESeq e1 e2) eff = Result id' res eff')
+   ->
+    (exists clock, fbs_single clock env id (ESeq e1' e2') eff = Result id' res eff')
+  ).
+  {
+    intros.
+    destruct H1. destruct x. inversion H1. simpl in H1.
+    destruct (fbs_expr x env id e0 eff) eqn:D1.
+    destruct res0. destruct v. congruence. destruct v0. 2, 4-5: congruence.
+    * epose (P := H _ _ _ _ _ _). destruct P. pose (P1 := H2 (ex_intro _ _ D1)).
+      epose (P := H0 _ _ _ _ _ _). destruct P. pose (P2 := H4 (ex_intro _ _ H1)).
+      destruct P1, P2. exists (S (x0 + x1)). simpl.
+      erewrite (bigger_clock_expr _ _ H6), (bigger_clock_expr _ _ H7). auto.
+      Unshelve. all: lia.
+    * epose (P := H _ _ _ _ _ _). destruct P. pose (P1 := H2 (ex_intro _ _ D1)). destruct P1.
+      exists (S x0). simpl. erewrite (bigger_clock_expr _ _ H4). auto. Unshelve. lia.
+  }
   split; intros.
-  * inversion H1; subst.
-    - eapply eval_seq. apply H. exact H6. auto. apply H0. exact H11.
-    - eapply eval_seq_ex. apply H. auto.
-  * inversion H1; subst.
-    - eapply eval_seq. apply H. exact H6. auto. apply H0. exact H11.
-    - eapply eval_seq_ex. apply H. auto.
+  * eapply A. exact H. exact H0. auto.
+  * eapply A. exact (fully_equivalent_expr_sym H). exact (fully_equivalent_expr_sym H0). auto.
 Qed.
 
-Theorem ELetRec_congr (exp : Expression) l : forall (exp' : Expression),
-  fully_equivalent exp exp'
+Theorem ELetRec_full_cong (exp : Expression) l : forall (exp' : Expression),
+  fully_equivalent_expr exp exp'
 ->
   fully_equivalent_single (ELetRec l exp) (ELetRec l exp').
 Proof.
-  intros. unfold fully_equivalent, fully_equivalent_single in *.
+  intros.
   split; intros.
-  * inversion H0. subst. eapply eval_letrec. apply H. exact H9.
-  * inversion H0. subst. eapply eval_letrec. apply H. exact H9.
+  * destruct H0, x. inversion H0. simpl in H0.
+    epose (P := H _ _ _ _ _ _). destruct P. pose (P := H1 (ex_intro _ _ H0)). destruct P.
+    exists (S x0). simpl. auto.
+  * destruct H0, x. inversion H0. simpl in H0.
+    epose (P := H _ _ _ _ _ _). destruct P. pose (P := H2 (ex_intro _ _ H0)). destruct P.
+    exists (S x0). simpl. auto.
 Qed.
 
-Theorem EMap_congr (l : list (Expression * Expression)) : 
+Theorem EMap_full_cong (l : list (Expression * Expression)) : 
   forall (l' : list (Expression * Expression)),
-  length l = length l' ->
-  (let exps := make_map_exps l in
-   let exps' := make_map_exps l' in
-  forall i, i < length exps -> fully_equivalent (nth i exps ErrorExp) (nth i exps' ErrorExp))
+  fully_equivalent_exprlist (make_map_exps l) (make_map_exps l')
 ->
   fully_equivalent_single (EMap l) (EMap l').
 Proof.
   assert (A :
     forall (l l' : list (Expression * Expression)) env id eff eff' id' res,
-    length l = length l' ->
-    (let exps := make_map_exps l in
-      let exps' := make_map_exps l' in
-       forall i, i < length exps -> fully_equivalent (nth i exps ErrorExp) (nth i exps' ErrorExp)) ->
-    |env, id, EMap l, eff | -s> |id', res, eff'|
+    fully_equivalent_exprlist (make_map_exps l) (make_map_exps l') ->
+    (exists clock, fbs_single clock env id (EMap l) eff = Result id' res eff')
     ->
-    |env, id, EMap l', eff | -s> |id', res, eff' |
-  ). {
-  intros. unfold fully_equivalent, fully_equivalent_single in *.
-  * inversion H1; subst; rewrite H in *.
-    - unfold exps, vals in *.
-      eapply eval_map.
-      + exact H3.
-      + exact H4.
-      + exact H5.
-      + exact H6.
-      + intros. rewrite length_make_map_exps in H2, H7. rewrite H in H7.
-        pose (H7 i H2). apply H0 in e. exact e.
-        rewrite length_make_map_exps. lia.
-      + exact H8.
-      + auto.
-      + auto.
-      + auto.
-    - unfold exps, vals in *.
-      eapply eval_map_ex.
-      + exact H3.
-      + exact H4.
-      + exact H5.
-      + reflexivity.
-      + exact H7.
-      + intros.
-        pose (H8 j H2). apply H0 in e. exact e.
-        rewrite length_make_map_exps. lia.
-      + apply H0 in H11. auto. rewrite length_make_map_exps. lia.
+    (exists clock, fbs_single clock env id (EMap l') eff = Result id' res eff')
+  ).
+  {
+    intros. unfold fully_equivalent_exprlist, fully_equivalent_single in *.
+    destruct H0. destruct x. inversion H0. simpl in H0.
+    destruct (fbs_values (fbs_expr x) env id (make_map_exps l0) eff) eqn:D.
+    destruct res0. 3-4: congruence.
+    * inversion H0. subst. epose (E := H _ _ _ _ _ _). destruct E.
+      pose (E := H1 (ex_intro _ x D)). destruct E. exists (S x0). simpl. rewrite H4. auto.
+    * inversion H0. subst. epose (E := H _ _ _ _ _ _). destruct E.
+      pose (E := H1 (ex_intro _ x D)). destruct E. exists (S x0). simpl. rewrite H3. auto.
   }
   split; intros.
-  * eapply A. exact H. auto. auto.
-  * eapply A. symmetry. exact H.
-    simpl. simpl in H0. rewrite length_make_map_exps. rewrite length_make_map_exps in H0.
-    intros. apply fully_equivalent_sym. apply H0. lia. auto.
+  * eapply A. exact H. auto.
+  * eapply A. exact (fully_equivalent_exprlist_sym H). auto.
 Qed.
 
-Theorem ETry_congr (e1 e2 e3 : Expression) vl1 vl2 : forall (e1' e2' e3' : Expression),
-  fully_equivalent e1 e1' ->
-  fully_equivalent e2 e2' ->
-  fully_equivalent e3 e3'
+Theorem ETry_full_cong (e1 e2 e3 : Expression) vl1 vl2 : forall (e1' e2' e3' : Expression),
+  fully_equivalent_expr e1 e1' ->
+  fully_equivalent_expr e2 e2' ->
+  fully_equivalent_expr e3 e3'
 ->
   fully_equivalent_single (ETry e1 vl1 e2 vl2 e3) (ETry e1' vl1 e2' vl2 e3').
 Proof.
-  assert (A : forall e1 e1' e2 e2' e3 e3' env id eff id' res eff',
-    fully_equivalent e1 e1' ->
-    fully_equivalent e2 e2' ->
-    fully_equivalent e3 e3' ->
-    |env, id, ETry e1 vl1 e2 vl2 e3, eff | -s> |id', res, eff'|
-    ->
-    |env, id, ETry e1' vl1 e2' vl2 e3', eff| -s> |id', res, eff'|
+  assert (A : forall env id id' res eff eff' e1 e1' e2 e2' e3 e3',
+    fully_equivalent_expr e1 e1' ->
+    fully_equivalent_expr e2 e2' ->
+    fully_equivalent_expr e3 e3' ->
+    (exists clock, fbs_single clock env id (ETry e1 vl1 e2 vl2 e3) eff = Result id' res eff')
+   ->
+    (exists clock, fbs_single clock env id (ETry e1' vl1 e2' vl2 e3') eff = Result id' res eff')
   ).
   {
-    intros. inversion H2; subst.
-    * eapply eval_try. apply H. exact H14. auto. apply H0. exact H16.
-    * eapply eval_catch. apply H. exact H14. apply H1. exact H15.
+    intros.
+    destruct H2. destruct x. inversion H2. simpl in H2.
+    destruct (fbs_expr x env id e0 eff) eqn:D1.
+    destruct res0. destruct (Datatypes.length v =? Datatypes.length vl1) eqn:D2.
+    2, 4-5: congruence.
+    * epose (P := H _ _ _ _ _ _). destruct P. pose (P1 := H3 (ex_intro _ _ D1)).
+      epose (P := H0 _ _ _ _ _ _). destruct P. pose (P2 := H5 (ex_intro _ _ H2)).
+      destruct P1, P2. exists (S (x0 + x1)). simpl.
+      erewrite (bigger_clock_expr _ _ H7), (bigger_clock_expr _ _ H8), D2. auto.
+      Unshelve. all: lia.
+    * epose (P := H _ _ _ _ _ _). destruct P. pose (P1 := H3 (ex_intro _ _ D1)).
+      epose (P := H1 _ _ _ _ _ _). destruct P. pose (P2 := H5 (ex_intro _ _ H2)).
+      destruct P1, P2. exists (S (x0 + x1)). simpl.
+      erewrite (bigger_clock_expr _ _ H7), (bigger_clock_expr _ _ H8). auto.
+      Unshelve. all: lia.
   }
   split; intros.
   * eapply A. exact H. exact H0. exact H1. auto.
-  * eapply A.
-    1-3: apply fully_equivalent_sym.
-    exact H. exact H0. exact H1. auto.
+  * eapply A. exact (fully_equivalent_expr_sym H). exact (fully_equivalent_expr_sym H0).
+    exact (fully_equivalent_expr_sym H1). auto.
 Qed.
 
-Theorem EValues_congr (l : list SingleExpression) : forall (l' : list SingleExpression),
-  length l = length l' ->
-  (forall i, i < length l -> fully_equivalent_single (nth i l ErrorExp) (nth i l' ErrorExp))
+Theorem EValues_full_cong (l : list SingleExpression) : forall (l' : list SingleExpression),
+  fully_equivalent_singlelist l l'
 ->
-  fully_equivalent (EValues l) (EValues l').
+  fully_equivalent_expr (EValues l) (EValues l').
 Proof.
   assert (A : forall (l l' : list SingleExpression) env id eff id' res eff',
-    length l = length l' ->
-    (forall i, i < length l -> fully_equivalent_single (nth i l ErrorExp) (nth i l' ErrorExp))
+    fully_equivalent_singlelist l l'
     ->
-    |env, id, EValues l, eff| -e> |id', res, eff'|
+    (exists clock, fbs_expr clock env id (EValues l) eff = Result id' res eff')
     ->
-    |env, id, EValues l', eff| -e> |id', res, eff'|). {
-  intros. unfold fully_equivalent, fully_equivalent_single in *.
-  * inversion H1; subst; rewrite H in *.
-    - eapply eval_values.
-      + exact H3.
-      + exact H4.
-      + exact H5.
-      + intros. pose (H6 i H2). apply H0 in e. 2: auto. auto.
-      + auto.
-      + auto.
-    - eapply eval_values_ex.
-      + exact H3.
-      + reflexivity.
-      + exact H5.
-      + exact H6.
-      + intros. pose (H7 j H2). apply H0 in e. 2: lia. auto.
-      + apply H0 in H10. auto. lia.
+    (exists clock, fbs_expr clock env id (EValues l') eff = Result id' res eff')).
+  {
+   intros. unfold fully_equivalent_exprlist, fully_equivalent_single in *.
+    destruct H0. destruct x. inversion H0. simpl in H0.
+    destruct (fbs_values (fbs_single x) env id l0 eff) eqn:D.
+    destruct res0. 3-4: congruence.
+    * inversion H0. subst. epose (E := H _ _ _ _ _ _). destruct E.
+      pose (E := H1 (ex_intro _ x D)). destruct E. exists (S x0). simpl. rewrite H3. auto.
+    * inversion H0. subst. epose (E := H _ _ _ _ _ _). destruct E.
+      pose (E := H1 (ex_intro _ x D)). destruct E. exists (S x0). simpl. rewrite H3. auto.
   }
   split; intros.
-  * eapply A. exact H. auto. auto.
-  * eapply A. symmetry. exact H. intros. rewrite <- H in *.
-    apply fully_equivalent_single_sym. auto. auto.
+  * eapply A. exact H. auto.
+  * eapply A. exact (fully_equivalent_singlelist_sym H). exact H0.
 Qed.
 
-Theorem ESingle_congr (e : SingleExpression)  : forall (e': SingleExpression),
+Theorem ESingle_full_cong (e : SingleExpression)  : forall (e': SingleExpression),
   fully_equivalent_single e e'
 ->
-  fully_equivalent (ESingle e) (ESingle e').
+  fully_equivalent_expr (ESingle e) (ESingle e').
 Proof.
-  unfold fully_equivalent_single.
+  intros.
   split; intros.
-  * inversion H0. eapply eval_single. subst. apply H. auto.
-  * inversion H0. eapply eval_single. subst. apply H. auto.
+  * destruct H0, x. inversion H0. simpl in H0.
+    epose (P := H _ _ _ _ _ _). destruct P. pose (P := H1 (ex_intro _ _ H0)). destruct P.
+    exists (S x0). simpl. auto.
+  * destruct H0, x. inversion H0. simpl in H0.
+    epose (P := H _ _ _ _ _ _). destruct P. pose (P := H2 (ex_intro _ _ H0)). destruct P.
+    exists (S x0). simpl. auto.
 Qed.
 
 End congruence.
@@ -785,46 +763,43 @@ end.
 
 Section examples.
 
-Example complete1 e :
-  fully_equivalent (e) (ESeq (ECall "+" [^ELit (Integer 2); ^ELit (Integer 2)]) e).
+(** 
+  * Examples why list congruence and list element congruence works only in one direction
+  * *)
+Goal
+  fully_equivalent_single (ETuple [^EApp ErrorExp []]) (ETuple [^ErrorExp;^EApp ErrorExp []]).
 Proof.
-  split; intros.
-  * constructor. econstructor.
-    - solve.
-    - exact H.
-  * inversion H. inversion H3. subst.
-    - inversion H12. inversion H4. subst.
-      simpl in H11, H13, H14.
-      unfold_list_once. inversion H1. clear H1.
-      unfold_list_once. inversion H1. clear H1.
-      unfold_list_once. unfold_list_once.
-      unfold_list_once. unfold_list_once. unfold_list_once.
-      unfold_list_once. unfold_list_once. unfold_list_once.
-      unfold_list_once. unfold_list_once. unfold_list_once.
-      inversion H2. subst. inversion H1. subst. inversion H5. subst.
-      epose (H15 0 (Nat.lt_0_2)). simpl in e0. inversion e0. subst. inversion H9. subst.
-      epose (H15 1 (Nat.lt_1_2)). simpl in e1. inversion e1. inversion H10. subst.
-      simpl in H17. inversion H19. subst. assumption.
-    - inversion H16. inversion H20; subst.
-      + simpl in H27, H28, H29.
-        unfold_list_once. inversion H1. clear H1.
-        unfold_list_once. inversion H1. clear H1.
-        unfold_list_once. unfold_list_once.
-        unfold_list_once. unfold_list_once. unfold_list_once.
-        unfold_list_once. unfold_list_once. unfold_list_once.
-        unfold_list_once. unfold_list_once. unfold_list_once.
-        inversion H4. inversion H2. inversion H1. subst.
-        epose (H30 0 (Nat.lt_0_2)). simpl in e0. inversion e0. subst. inversion H8. subst.
-        epose (H30 1 (Nat.lt_1_2)). simpl in e1. inversion e1. inversion H9. subst.
-        inversion H33.
-      + inversion H28. rewrite H1 in *.
-        ** unfold_list_once. unfold_list_once. unfold_list_once.
-           unfold_list_once. unfold_list_once. unfold_list_once. unfold_list_once.
-           unfold_list_once. unfold_list_once. inversion H2. inversion H0. inversion H1.
-           subst. inversion H38. inversion H7.
-        ** inversion H1. 2: inversion H4.
-           rewrite H4 in *. unfold_list_once. unfold_list_once. unfold_list_once.
-           inversion H38. inversion H5.
+  split; intros; destruct H; destruct x; inversion H.
+  * clear H1. exists (S x).
+    simpl in H; destruct x; inversion H.
+    simpl in H; destruct x; inversion H.
+    simpl in H; destruct x; inversion H.
+    simpl in H; destruct x; inversion H. simpl in H. inversion H. clear H1. clear H2. clear H3.
+    simpl. auto.
+  * clear H1. exists (S x).
+    simpl in H; destruct x; inversion H.
+    simpl in H; destruct x; inversion H.
+    simpl in H; destruct x; inversion H.
+    simpl in H; destruct x; inversion H. simpl in H. inversion H. clear H1. clear H2. clear H3.
+    simpl. auto.
 Qed.
+
+(** 
+  * The pair of the prevoius example
+  *)
+
+Goal
+  fully_equivalent_single (ETuple [^ErrorExp; ^EApp ErrorExp []]) (ETuple [^ErrorExp;^EApp ErrorExp []]).
+Proof.
+  apply ETuple_full_cong. apply fully_equivalent_elements_exprlist; auto.
+  intros. inversion H. 2: inversion H1. 3: inversion H3.
+  all: apply fully_equivalent_expr_refl.
+Qed.
+
+Example complete1 e :
+  fully_equivalent_expr (e) (ESeq (ECall "+" [^ELit (Integer 2); ^ELit (Integer 2)]) e).
+Proof.
+  
+Admitted.
 
 End examples.
